src/axiomatic/PFtoA4Atomic.v
@@ -43,7 +43,7 @@ Lemma sim_traces_sim_th'_atomic
       (RF2: Valid.rf2 ex)
       (RF_WF: Valid.rf_wf ex)
       (TR: IdMap.Forall2
-             (fun _ tr sl => exists l, tr = (ExecUnit.mk sl.(fst) sl.(snd) m.(Machine.mem)) :: l)
+             (fun _ tr sl => exists l, tr = (ExecUnit.mk (fst sl) (snd sl) m.(Machine.mem)) :: l)
              trs m.(Machine.tpool))
       (ATR: IdMap.Forall2
               (fun _ atr aeu => exists l, atr = aeu :: l)
