src/axiomatic/PFtoA4OBR.v
@@ -36,14 +36,14 @@ Lemma sim_traces_sim_th'_ob_read
       (PRE: Valid.pre_ex p ex)
       (CO: ex.(Execution.co) = co_gen ws)
       (RF: ex.(Execution.rf) = rf_gen ws rs)
-      (INTERNAL: acyclic ex.(Execution.internal))
+      (INTERNAL: acyclic (Execution.internal ex))
       (CO1: Valid.co1 ex)
       (CO2: Valid.co2 ex)
       (RF1: Valid.rf1 ex)
       (RF2: Valid.rf2 ex)
       (RF_WF: Valid.rf_wf ex)
       (TR: IdMap.Forall2
-             (fun _ tr sl => exists l, tr = (ExecUnit.mk sl.(fst) sl.(snd) m.(Machine.mem)) :: l)
+             (fun _ tr sl => exists l, tr = (ExecUnit.mk (fst sl) (snd sl) m.(Machine.mem)) :: l)
              trs m.(Machine.tpool))
       (ATR: IdMap.Forall2
               (fun _ atr aeu => exists l, atr = aeu :: l)
